tests/lean/run/grind_constProp.lean
@@ -82,10 +82,10 @@ attribute [local grind] State.update State.find? State.get State.erase
   grind
 
 @[simp] theorem State.find?_update_self (σ : State) (x : Var) (v : Val) : (σ.update x v).find? x = some v := by
-  induction σ, x, v using State.update.induct <;> grind
+  induction σ using State.update.induct x <;> grind
 
 @[simp] theorem State.find?_update (σ : State) (v : Val) (h : x ≠ z) : (σ.update x v).find? z = σ.find? z := by
-  induction σ, x, v using State.update.induct <;> grind
+  induction σ using State.update.induct x <;> grind
 
 @[grind =] theorem State.find?_update_eq (σ : State) (v : Val)
     : (σ.update x v).find? z = if x = z then some v else σ.find? z := by
@@ -95,17 +95,17 @@ attribute [local grind] State.update State.find? State.get State.erase
   grind
 
 @[simp] theorem State.find?_erase_self (σ : State) (x : Var) : (σ.erase x).find? x = none := by
-  induction σ, x using State.erase.induct <;> grind
+  induction σ using State.erase.induct x <;> grind
 
 @[simp] theorem State.find?_erase (σ : State) (h : x ≠ z) : (σ.erase x).find? z = σ.find? z := by
-  induction σ, x using State.erase.induct <;> grind
+  induction σ using State.erase.induct x <;> grind
 
 @[simp, grind =] theorem State.find?_erase_eq (σ : State)
     : (σ.erase x).find? z = if x = z then none else σ.find? z := by
   grind only [= find?_erase_self, = find?_erase, cases Or]
 
 @[grind] theorem State.length_erase_le (σ : State) (x : Var) : (σ.erase x).length ≤ σ.length := by
-  induction σ, x using erase.induct <;> grind
+  induction σ using erase.induct x <;> grind
 
 def State.length_erase_lt (σ : State) (x : Var) : (σ.erase x).length < σ.length.succ := by
   grind
