tests/lean/run/structuralMutual.lean
@@ -449,14 +449,13 @@ inductive T (n : Nat) : Nat → Type where
   | n : T n n → T n n
 
 /--
-error: cannot use specified measure for structural recursion:
-  its type is an inductive datatype
-    T n n
-  and the datatype parameter
+error: failed to infer structural recursion:
+Cannot use parameter #2:
+  its type is an inductive datatype and the datatype parameter
     n
   depends on the function parameter
     n
-  which does not come before the varying parameters and before the indices of the recursion parameter.
+  which cannot be fixed as it is in a index, or depends on on index, and indices cannot be fixed parameters with structural recursion.
 -/
 #guard_msgs in
 def T.a {n : Nat} : T n n → Nat
@@ -514,13 +513,13 @@ Too many possible combinations of parameters of type Nattish (or please indicate
 Could not find a decreasing measure.
 The basic measures relate at each recursive call as follows:
 (<, ≤, =: relation proved, ? all proofs failed, _: no proof attempted)
-Call from ManyCombinations.f to ManyCombinations.g at 546:15-29:
+Call from ManyCombinations.f to ManyCombinations.g at 545:15-29:
    #1 #2 #3 #4
 #5  ?  ?  ?  ?
 #6  ?  ?  =  ?
 #7  ?  ?  ?  =
 #8  ?  =  ?  ?
-Call from ManyCombinations.g to ManyCombinations.f at 549:15-29:
+Call from ManyCombinations.g to ManyCombinations.f at 548:15-29:
    #5 #6 #7 #8
 #1  _  _  _  _
 #2  _  _  _  ?
